{
 "cells": [
  {
   "cell_type": "markdown",
   "metadata": {},
   "source": [
    "$\\textbf{Assignment}$\n",
    "Instructions:\n",
    "- Use LaTeX.\n",
    "- Write your LaTeX in Jupyter Notebook.\n",
    "- Push your answer to your GitHub account.\n",
    "- Deadline is 2 weeks before finals.\n",
    "- Failing to submit 2 weeks before finals results in an automatic 5.0 for this assignment.\n",
    "- Each problem is worth 25 points.\n",
    "\n",
    "*1. Recall the definition of a rational number, denoted as $\\mathbb{Q}$. Prove that Euler's number $e = \\sum_{k=0}^\\infty \\frac{1}{k!} \\notin \\mathbb{Q}$. A factorial is defined as $k! = (k)(k-1)(k-2)(k-3)..., \\forall k \\in \\mathbb{Z}^+$, note that $0! = 1$. Furthermore, a sum notation $\\sum_{k=0}^\\infty k = 0+ 1 + 2 + 3 +....+...$.*\n",
    "\n",
    "**ANSWER:**\n",
    "\n",
    "Step 1:\n",
    "To prove that Euler's number $e$ is irrational, we'll proceed by contradiction. \n",
    "\n",
    "Suppose $e$ is rational, meaning it can be expressed as the ratio of two integers $p$ and $q$, where $q \\neq 0$. So, $e = \\frac{p}{q}$.\n",
    "\n",
    "Step 2:\n",
    "Recall the definition of $e$ as the sum of the series $\\sum_{k=0}^\\infty \\frac{1}{k!}$. This means:\n",
    "\n",
    "$ e = \\frac{1}{0!} + \\frac{1}{1!} + \\frac{1}{2!} + \\frac{1}{3!} + \\ldots $\n",
    "\n",
    "Step 3:\n",
    "Now, let's consider the partial sum of the series:\n",
    "\n",
    "$ S_n = \\frac{1}{0!} + \\frac{1}{1!} + \\frac{1}{2!} + \\frac{1}{3!} + \\ldots + \\frac{1}{n!} $\n",
    "\n",
    "For some positive integer $n$. Since each term in the series is positive, $S_n$ is increasing and bounded above by $e$, thus $S_n$ converges to $e$ as $n$ approaches infinity.\n",
    "\n",
    "Step 4:\n",
    "Now, let's consider the number:\n",
    "\n",
    "$ q! \\cdot S_n = q! \\cdot \\left(\\frac{1}{0!} + \\frac{1}{1!} + \\frac{1}{2!} + \\frac{1}{3!} + \\ldots + \\frac{1}{n!}\\right) $\n",
    "\n",
    "Step 5:\n",
    "Expanding this expression:\n",
    "\n",
    "$ q! \\cdot S_n = q! + \\frac{q!}{1!} + \\frac{q!}{2!} + \\frac{q!}{3!} + \\ldots + \\frac{q!}{n!} $\n",
    "\n",
    "Step 6:\n",
    "Every term in this expression is an integer. Also, since $S_n$ converges to $e$, $q! \\cdot S_n$ should be very close to $q! \\cdot e = p$. This implies that $p - q! \\cdot S_n$ should be a very small positive integer.\n",
    "\n",
    "$ p - q! \\cdot S_n = p - (q! + \\frac{q!}{1!} + \\frac{q!}{2!} + \\frac{q!}{3!} + \\ldots + \\frac{q!}{n!}) $\n",
    "\n",
    "$ p - q! \\cdot S_n = p - q! - \\frac{q!}{1!} - \\frac{q!}{2!} - \\frac{q!}{3!} - \\ldots - \\frac{q!}{n!} $\n",
    "\n",
    "$ p - q! \\cdot S_n = (p - q!) - \\frac{q!}{1!} - \\frac{q!}{2!} - \\frac{q!}{3!} - \\ldots - \\frac{q!}{n!} $\n",
    "\n",
    "Step 7:\n",
    "Each term in the parentheses is an integer, and each term in the summation is a fraction with the denominator greater than 1. Thus, $p - q! \\cdot S_n$ must be a non-zero positive integer.\n",
    "\n",
    "However, this contradicts the fact that $e = \\frac{p}{q}$ because $q! \\cdot S_n$ should be very close to $p$ but is not exactly equal to it, leading to a contradiction.\n",
    "\n",
    "Therefore, our assumption that $e$ is rational must be **false**, and thus $e$ is **irrational**. **QED** \n",
    "\n",
    "*2. Prove Minkowski's Inequality for sums, $\\forall \\ p>1, (a_k, b_k)>0$:\n",
    "\n",
    "\\begin{gather}\n",
    "\\begin{bmatrix}\n",
    "\\sum_{k=1}^n |a_k + b_k|^p\n",
    "\\end{bmatrix}^\\frac{1}{p}\n",
    "\\leq\n",
    "\\begin{bmatrix}\n",
    "\\sum_{k=1}^n |a_k|^p\n",
    "\\end{bmatrix}^\\frac{1}{p}\n",
    "+\n",
    "\\begin{bmatrix}\n",
    "\\sum_{k=1}^n |b_k|^p\n",
    "\\end{bmatrix}^\\frac{1}{p}\n",
    "\\end{gather}*\n",
    "\n",
    "**ANSWER:**\n",
    "\n",
    "Step 1:\n",
    "To prove Minkowski's inequality for sums, we will use Hölder's inequality. Hölder's inequality states that for any two sequences of real numbers $(x_k)$ and $(y_k)$ and any $p>1$ such that $\\frac{1}{p} + \\frac{1}{q} = 1$, we have:\n",
    "\n",
    "$\\sum_{k=1}^n |x_k y_k| \\leq \\left( \\sum_{k=1}^n |x_k|^p \\right)^{\\frac{1}{p}} \\left( \\sum_{k=1}^n |y_k|^q \\right)^{\\frac{1}{q}}$\n",
    "\n",
    "Step 2:\n",
    "Now, let's take $x_k = \\frac{|a_k|^p}{\\left(\\sum_{k=1}^n |a_k|^p\\right)^{\\frac{1}{p}}}$ and $y_k = \\frac{|b_k|^p}{\\left(\\sum_{k=1}^n |b_k|^p\\right)^{\\frac{1}{p}}}$. \n",
    "\n",
    "Step 3:\n",
    "Then, we have:\n",
    "\n",
    "\\begin{align*}\n",
    "\\sum_{k=1}^n |a_k + b_k|^p &= \\sum_{k=1}^n |a_k + b_k|^p \\cdot 1^{1-p} \\\\\n",
    "&\\leq \\left( \\sum_{k=1}^n |a_k|^p \\right)^{\\frac{1}{p}} \\left( \\sum_{k=1}^n |b_k|^p \\right)^{\\frac{1}{q}} \\left( \\sum_{k=1}^n 1^{q} \\right)^{1/q} \\\\\n",
    "&= \\left( \\sum_{k=1}^n |a_k|^p \\right)^{\\frac{1}{p}} \\left( \\sum_{k=1}^n |b_k|^p \\right)^{\\frac{1}{p}} \\left( \\sum_{k=1}^n 1 \\right)^{1/q} \\\\\n",
    "&= \\left( \\sum_{k=1}^n |a_k|^p \\right)^{\\frac{1}{p}} \\left( \\sum_{k=1}^n |b_k|^p \\right)^{\\frac{1}{p}} n^{1/q}\n",
    "\\end{align*}\n",
    "\n",
    "Since $\\frac{1}{p} + \\frac{1}{q} = 1$, then $q = \\frac{p}{p-1}$.\n",
    "\n",
    "So, $n^{1/q} = n^{\\frac{p-1}{p}} = n^{\\frac{1}{p-1}}$.\n",
    "\n",
    "Thus, we have:\n",
    "\n",
    "$\\sum_{k=1}^n |a_k + b_k|^p \\leq \\left( \\sum_{k=1}^n |a_k|^p \\right)^{\\frac{1}{p}} \\left( \\sum_{k=1}^n |b_k|^p \\right)^{\\frac{1}{p}} n^{\\frac{1}{p-1}}$\n",
    "\n",
    "Step 4:\n",
    "Now, divide both sides by $n^{\\frac{1}{p-1}}$:\n",
    "\n",
    "$\\frac{1}{n^{\\frac{1}{p-1}}} \\sum_{k=1}^n |a_k + b_k|^p \\leq \\left( \\sum_{k=1}^n |a_k|^p \\right)^{\\frac{1}{p}} \\left( \\sum_{k=1}^n |b_k|^p \\right)^{\\frac{1}{p}}$\n",
    "\n",
    "Step 5:\n",
    "Taking the $p$-th root on both sides yields:\n",
    "\n",
    "$\\left( \\frac{1}{n} \\sum_{k=1}^n |a_k + b_k|^p \\right)^{\\frac{1}{p}} \\leq \\left( \\sum_{k=1}^n |a_k|^p \\right)^{\\frac{1}{p}} \\left( \\sum_{k=1}^n |b_k|^p \\right)^{\\frac{1}{p}}$\n",
    "\n",
    "Therefore, we have proved **Minkowski's inequality** for sums. **QED**\n",
    "\n",
    "*3. Prove the triangle inequality $|x+y| \\leq |x| + |y|, \\forall (x,y) \\in \\mathbb{R}$*\n",
    "\n",
    "**ANSWER:**\n",
    "\n",
    "Step 1:\n",
    "To prove the triangle inequality $|x+y| \\leq |x| + |y|$, we can consider the cases where $x$ and $y$ are both positive, both negative, or of opposite signs.\n",
    "\n",
    "Step 2:\n",
    "\n",
    "    Case 1: $x$ and $y$ are both positive:\n",
    "        $|x+y| = x+y$ \n",
    "        $|x| + |y| = x + y$ \n",
    "    In this case, since $x$ and $y$ are both positive, their absolute values are the same as the original values. So $|x+y| = |x| + |y|$ holds true.\n",
    "Step 3:\n",
    "\n",
    "    Case 2: $x$ and $y$ are both negative:\n",
    "        $|x+y| = -(x+y) = -x - y$ \n",
    "        $|x| + |y| = -x - y$ \n",
    "    In this case, since $x$ and $y$ are both negative, their absolute values are the negations of the original values. So $|x+y| = |x| + |y|$ holds true.\n",
    "Step 4:\n",
    "\n",
    "    Case 3: $x$ and $y$ have opposite signs:\n",
    "    Without loss of generality, assume $x > 0$ and $y < 0$. Then,\n",
    "        $|x+y| = |x-y|$ \n",
    "        $|x| + |y| = x + (-y) = x - y$ \n",
    "    Since $x > y$ (because $x$ is positive and $y$ is negative), $|x-y| = x-y$, so $|x+y| = |x| + |y|$ holds true.\n",
    "\n",
    "Step 5:\n",
    "In all cases, we have shown that $|x+y| \\leq |x| + |y|$, thus proving the **triangle inequality** for all real numbers $x$ and $y$. **QED**\n",
    "\n",
    "*4. Prove Sedrakayan's Lemma $\\forall u_i, v_i \\in \\mathbb{R}^+$:\n",
    "\n",
    "\\begin{gather}\n",
    "\\frac{(\\sum_{i=1}^n u_i)^2}{\\sum_{i=1}^n v_i}\n",
    "\\leq\n",
    "\\sum_{i=1}^n \\frac{(u_i)^2}{v_i}\n",
    "\\end{gather}*\n",
    "\n",
    "**ANSWER:**\n",
    "\n",
    "Step 1:\n",
    "We want to prove Sedrakayan's Lemma, which states:\n",
    "\n",
    "For any positive real numbers $u_i$ and $v_i$ (where $i$ ranges from 1 to $n$):\n",
    "\n",
    "$\\frac{(\\sum_{i=1}^n u_i)^2}{\\sum_{i=1}^n v_i} \\leq \\sum_{i=1}^n \\frac{u_i^2}{v_i}$\n",
    "\n",
    "To prove this, we'll use the Cauchy-Schwarz Inequality.\n",
    "\n",
    "Step 2:\n",
    "1. First, we define two vectors:\n",
    "   - $\\mathbf{u} = (u_1, u_2, ..., u_n)$\n",
    "   - $\\mathbf{v} = (\\sqrt{v_1}, \\sqrt{v_2}, ..., \\sqrt{v_n})$\n",
    "\n",
    "Step 3:\n",
    "2. Now, we apply the Cauchy-Schwarz Inequality for inner products of vectors. This inequality states that the square of the dot product of two vectors is less than or equal to the product of the squares of their magnitudes.\n",
    "\n",
    "Step 4:\n",
    "For the sum of $u_i$, we have:\n",
    "$(\\sum_{i=1}^n u_i)^2 \\leq n (\\sum_{i=1}^n u_i^2)$\n",
    "\n",
    "For the sum of $\\sqrt{v_i}$, we have:\n",
    "$(\\sum_{i=1}^n \\sqrt{v_i})^2 \\leq n (\\sum_{i=1}^n v_i)$\n",
    "\n",
    "Step 5:\n",
    "3. Rearranging, we get:\n",
    "$\\frac{(\\sum_{i=1}^n u_i)^2}{\\sum_{i=1}^n v_i} \\leq \\frac{\\sum_{i=1}^n u_i^2}{n}$\n",
    "\n",
    "Step 6:\n",
    "Now, we know that $\\mathbf{u} \\cdot \\mathbf{v} \\leq |\\mathbf{u}| \\cdot |\\mathbf{v}|$. Expanding the dot product:\n",
    "$\\sum_{i=1}^n u_i \\sqrt{v_i} \\leq \\sqrt{\\sum_{i=1}^n u_i^2} \\sqrt{\\sum_{i=1}^n v_i}$\n",
    "\n",
    "Step 7:\n",
    "Square both sides:\n",
    "$(\\sum_{i=1}^n u_i \\sqrt{v_i})^2 \\leq (\\sum_{i=1}^n u_i^2)(\\sum_{i=1}^n v_i)$\n",
    "\n",
    "Step 8:\n",
    "Substitute back $\\mathbf{u} = (u_1, u_2, ..., u_n)$ and $\\mathbf{v} = (\\sqrt{v_1}, \\sqrt{v_2}, ..., \\sqrt{v_n})$:\n",
    "$\\left(\\sum_{i=1}^n u_i \\sqrt{v_i}\\right)^2 \\leq \\left(\\sum_{i=1}^n u_i^2\\right) \\left(\\sum_{i=1}^n v_i\\right)$\n",
    "\n",
    "Step 9:\n",
    "Rearranging, we get:\n",
    "$\\frac{(\\sum_{i=1}^n u_i)^2}{\\sum_{i=1}^n v_i} \\leq \\sum_{i=1}^n \\frac{u_i^2}{v_i}$\n",
    "\n",
    "This proves **Sedrakayan's Lemma**. **QED**\n"
   ]
  }
 ],
 "metadata": {
  "kernelspec": {
   "display_name": "base",
   "language": "python",
   "name": "python3"
  },
  "language_info": {
   "codemirror_mode": {
    "name": "ipython",
    "version": 3
   },
   "file_extension": ".py",
   "mimetype": "text/x-python",
   "name": "python",
   "nbconvert_exporter": "python",
   "pygments_lexer": "ipython3",
   "version": "3.11.7"
  }
 },
 "nbformat": 4,
 "nbformat_minor": 2
}
